Proved Laws for state monad; slightly weaker bind inversion rule

theories/Basics/MonadState.v
@@ -29,8 +29,16 @@ Section State.
     s ~~> prod_typ s a.
 
   Definition eqmR_state (A B : typ) (R : relationH A B) :=
-    (fun (p : state S A × state S B) =>
-        forall s, S ⊗ R @ (fst p @ s, snd p @ s)).
+    (fun (p : state S A × state S B) => forall (s : S),
+      (* Weak equivalence on R *)
+      ((forall (a : A), snd (fst p @ s) == a ->
+        (exists (b : B), R @ (a, b) /\ snd (snd p @ s) == b)) /\
+        (forall (b : B), snd (snd p @ s) == b ->
+        (exists (a : A), R @ (a, b) /\ snd (fst p @ s) == a))) /\
+      (* Equivalence on resulting state *)
+      ((relationH_of_typ S) @ (fst (fst p @ s), fst (snd p @ s)))).
+
+  Lemma equal_typ {A : typ} {x : A} : x == x. reflexivity. Qed.
 
   Program Instance EqmR_state : EqmR (state S) :=
     {
@@ -38,110 +46,157 @@ Section State.
     }.
   Next Obligation.
     repeat intro. destruct x2, y. cbn in *. destruct H.
-    unfold eqmR_state. cbn. split. intros.
-    specialize (H1 s).
-    specialize (H s s).
-    assert (s == s) by reflexivity.
-    specialize (H H2). specialize (H0 s s H2).
-    destruct (t @ s). destruct (t0 @ s). destruct (t1 @ s). destruct (t2 @ s).
-    destruct H, H0. cbn in *; destruct H1. rewrite <- H. rewrite <- H0.
-    split. auto. rewrite <- H3. rewrite <- H4. auto.
-    intros.
-    specialize (H1 s).
-    specialize (H s s).
-    assert (s == s) by reflexivity.
-    specialize (H H2). specialize (H0 s s H2).
-    destruct (t @ s). destruct (t0 @ s). destruct (t1 @ s). destruct (t2 @ s).
-    destruct H, H0. cbn in *; destruct H1. rewrite H. rewrite H0.
-    split. auto. rewrite H3. rewrite H4. auto.
+    unfold eqmR_state. cbn. split.
+    - intros.
+      specialize (H1 s).
+      specialize (H s s).
+      assert (s == s) by reflexivity.
+      specialize (H H2). specialize (H0 s s H2).
+      destruct (t @ s). destruct (t0 @ s). destruct (t1 @ s). destruct (t2 @ s).
+      destruct H, H0. intuition; cbn in *.
+      intuition. edestruct H1; eauto. rewrite H5 in H8.
+      destruct H8. exists (x2). split; eauto. rewrite <- H4; auto.
+      edestruct H7; eauto. rewrite H5 in H8. destruct H8.
+      exists x2; split; auto. rewrite <- H9; symmetry; auto.
+      rewrite <- H0. rewrite <- H6. symmetry; auto.
+    - intros.
+      specialize (H1 s).
+      specialize (H s s).
+      assert (s == s) by reflexivity.
+      specialize (H H2). specialize (H0 s s H2).
+      destruct (t @ s). destruct (t0 @ s). destruct (t1 @ s). destruct (t2 @ s).
+      destruct H, H0. intuition; cbn in *.
+      intuition. edestruct H1. symmetry; eauto.
+      rewrite H5 in H8.
+      destruct H8. exists (x2). split; eauto. rewrite H4; auto.
+      edestruct H7; eauto. symmetry; eauto.
+      rewrite H5 in H8. destruct H8.
+      exists x2; split; auto. rewrite <- H9; auto.
+      symmetry; auto. rewrite H0. rewrite <- H6. symmetry; auto.
   Qed.
   Next Obligation.
     split; repeat intro. cbn in *. rewrite H0.
     - unfold eqmR_state in H.
       specialize (H x0).
-      change (S ⊗ A @ (x @ x0, y @ x0)) in H.
-      rewrite <- H0. destruct (x @ x0). destruct (y @ x0).
-      cbn in *. apply H.
-    - change (S ⊗ A @ (x @ s, y @ s)).
-      unfold state in *.
-      repeat red in H. cbn in H. specialize (H s s).
-      assert (s == s) by reflexivity.
-      specialize (H H0). destruct (x @ s). destruct (y @ s).
-      cbn in *. apply H.
+      destruct H. destruct H. setoid_rewrite H0 in H.
+      setoid_rewrite H0 in H2.
+      setoid_rewrite H0 in H1.
+      cbn in *. destruct (x @ y0) eqn: Hx. destruct (y @ y0) eqn: Hy. cbn in *.
+      split. apply H1. specialize (H2 t2).
+      specialize (H2 equal_typ).
+      edestruct H2 as (? & ? & ?). rewrite H4. auto.
+    - unfold eqmR_state in H.
+      specialize (H s s equal_typ).
+      cbn in *. destruct (x @ s) eqn: Hx. destruct (y @ s) eqn: Hy. cbn in *.
+      destruct H. split. split.
+      intros. exists t0. split; symmetry; auto.
+      intros. exists t2; split; auto. auto.
   Qed.
-
-  Lemma equal_typ {s} : s == s. reflexivity. Qed.
 
   Instance EqmR_OK_state : EqmR_OK (state S).
   constructor.
   - intros. repeat intro. unfold ReflexiveH in H.
-    change (S ⊗ R @ (a @ s, a @ s)).
-    unfold state in a.
-    destruct (a @ s). cbn in *. split. reflexivity. auto.
+    cbn. split. split. intros. exists a0. split; eauto.
+    intros. eauto. reflexivity.
   - intros. repeat intro. unfold SymmetricH in H.
-    destruct p.
-    change (S ⊗ R @ (t0 @ s, t @ s)).
-    cbn in H0. unfold eqmR_state in H0.
+    destruct p. cbn. cbn in H0.
+    unfold eqmR_state in H0. cbn in H0.
     specialize (H0 s).
-    change (S ⊗ R @ (t @ s, t0 @ s)) in H0.
-    destruct (t0 @ s). destruct (t @ s).
-    cbn in *. destruct H0. split. symmetry. apply H0.
-    specialize (H (t4, t2) H1). apply H.
+    destruct H0. destruct H0. split. split.
+    intros. edestruct H2. apply H3. destruct H4.
+    edestruct H0. apply H5. destruct H6. exists x. split; auto.
+    specialize (H (x, a) H4). cbn in H. auto.
+    intros. edestruct H0. apply H3. destruct H4.
+    edestruct H2. apply H5. destruct H6. exists x. split; auto.
+    specialize (H (b, x) H4). cbn in H. auto.
+    symmetry; auto.
   - intros. repeat intro. unfold TransitiveH in H.
     destruct p, q. cbn in H2. red in H2.
     specialize (H2 s s equal_typ).
-    change (S ⊗ R @ (t @ s, t2 @ s)).
-    cbn in H0, H1; unfold eqmR_state in H0, H1.
+    cbn in *. unfold eqmR_state in *. cbn in *.
     specialize (H0 s). specialize (H1 s).
-    change (S ⊗ R @ (t @ s, t0 @ s)) in H0.
-    change (S ⊗ R @ (t1 @ s, t2 @ s)) in H1.
-    rewrite H2 in H0. clear H2; clear t0.
-    destruct (t @ s), (t1 @ s), (t2 @ s).
-    cbn in *. destruct H0, H1. split. etransitivity; eauto.
-    specialize (H (t3, t5) (t5, t7) H2 H3). apply H. reflexivity.
-  - repeat intro. cbn in H, H0. unfold eqmR_state in H, H0.
-    specialize (H s); specialize (H0 s).
-    change (S ⊗ R1 @ (ma @ s, mb @ s)) in H.
-    change (S ⊗ R2 @ (mb @ s, mc @ s)) in H0.
-    change (S ⊗ (R2 ∘ R1) @ (ma @ s, mc @ s)).
-    destruct (ma @ s), (mb @ s), (mc @ s).
-    cbn in *. destruct H, H0. split. etransitivity; eauto.
-    exists t2. split; eauto.
+    destruct H2. destruct (t @ s), (t0 @ s), (t1 @ s), (t2 @ s).
+    cbn in *. destruct H0. destruct H0. destruct H1. destruct H1.
+    split. split.
+    + intros. edestruct H1. symmetry; eauto.
+      destruct H9. edestruct H0. apply H8. destruct H11.
+      edestruct H5. apply H12. destruct H13. cbn in *.
+      edestruct H7. apply H10. destruct H15. exists x. split; auto.
+      rewrite H12 in H9. specialize (H (a, x0) (x0, x) H11 H9).
+      cbn in H. specialize (H equal_typ). auto.
+    + intros. edestruct H7; eauto. destruct H9.
+      edestruct H1; eauto. destruct H11.
+      edestruct H5; eauto. destruct H13. edestruct H0; eauto.
+      destruct H15. rewrite <- H10 in H9.
+      specialize (H (x1, t8) (t8, b) H13 H9).
+      cbn in H.
+      exists x1. split; intuition.
+    + rewrite H4. rewrite H2. auto.
+  - intros. cbn in *. unfold eqmR_state in *.
+    intros. specialize (H s). specialize (H0 s).
+    destruct H. destruct H. destruct H0. destruct H0. cbn in *.
+    split. split.
+    + intros. specialize (H a H5). edestruct H as (? & ? & ?); clear H.
+      destruct (ma @ s), (mb @ s), (mc @ s). cbn in *.
+      specialize (H2 _ H7). edestruct H2 as (? & ? & ?); clear H2.
+      specialize (H0 _ H7). edestruct H0 as (? & ? & ?); clear H0.
+      exists x1. split; intuition. exists x. split; intuition.
+    + intros. specialize (H4 _ H5). edestruct H4 as (? & ? & ?); clear H4.
+      destruct (ma @ s), (mb @ s), (mc @ s). cbn in *.
+      specialize (H2 _ H7). edestruct H2 as (? & ? & ?); clear H2.
+      exists x0. split; auto. exists x. split; auto.
+    + destruct (ma @ s), (mb @ s), (mc @ s). cbn in *.
+      rewrite H1. auto.
   - intros. split; repeat intro.
-    cbn in H; unfold eqmR_state in H.
-    specialize (H s).
-    change (S ⊗ † R @ (x @ s, y @ s)) in H.
-    change (S ⊗ R @ (y @ s, x @ s)).
-    destruct (x @ s), (y @ s).
-    cbn in *. destruct H; split. symmetry; auto. auto.
-    cbn in H; unfold eqmR_state in H.
-    specialize (H s).
-    change (S ⊗ R @ (y @ s, x @ s)) in H.
-    change (S ⊗ † R @ (x @ s, y @ s)).
-    destruct (x @ s), (y @ s).
-    cbn in *. destruct H; split. symmetry; auto. auto.
-  - repeat intro.
-    red in H. destruct H. red in H, H0.
-    split; repeat intro.
-    + change (S ⊗ y @ (x0 @ s, y0 @ s)).
-      cbn in H1. unfold eqmR_state in H1.
-      specialize (H1 s).
-      change (S ⊗ x @ (x0 @ s, y0 @ s)) in H1.
-      destruct (x0 @ s), (y0 @ s).
-      cbn in *. destruct H1. split; auto.
-    + change (S ⊗ x @ (x0 @ s, y0 @ s)).
-      cbn in H1. unfold eqmR_state in H1.
-      specialize (H1 s).
-      change (S ⊗ y @ (x0 @ s, y0 @ s)) in H1.
-      destruct (x0 @ s), (y0 @ s).
-      cbn in *. destruct H1. split; auto.
-  - repeat intro.
-    cbn in H0; unfold eqmR_state in H0.
-    specialize (H0 s). red in H.
-    change (S ⊗ y @ (x0 @ s, y0 @ s)).
-    change (S ⊗ x @ (x0 @ s, y0 @ s)) in H0.
-    destruct (x0 @ s), (y0 @ s). cbn in *.
-    destruct H0. split; auto.
+    + cbn in H. unfold eqmR_state in H. cbn in *.
+      specialize (H s). destruct H. destruct H.
+      destruct (x @ s), (y @ s); cbn in *.
+      split. split.
+      * intros. specialize (H1 _ H2). edestruct H1 as (? & ? & ?).
+        exists x0. split; auto.
+      * intros. specialize (H _ H2). edestruct H as (? & ? & ?).
+        exists x0. split; auto.
+      * symmetry; auto.
+    + cbn in H. unfold eqmR_state in H. cbn in *.
+      specialize (H s). destruct H. destruct H.
+      destruct (x @ s), (y @ s); cbn in *.
+      split. split.
+      * intros. specialize (H1 _ H2). edestruct H1 as (? & ? & ?).
+        exists x0. split; auto.
+      * intros. specialize (H _ H2). edestruct H as (? & ? & ?).
+        exists x0. split; auto.
+      * symmetry; auto.
+  - repeat intro. cbn in *. unfold eqmR_state.
+    split; repeat intro. cbn in H0.
+    + specialize (H0 s). cbn. destruct (x0 @ s), (y0 @ s). cbn in *.
+      red in H. destruct H. red in H, H1.
+      destruct H0. destruct H0.
+      split. split.
+      * intros. specialize (H0 _ H4). edestruct H0 as (? & ? & ?); clear H0.
+        exists x1. split; auto.
+      * intros. specialize (H3 _ H4). edestruct H3 as (? & ? & ?); clear H0.
+        exists x1. split; auto.
+      * auto.
+    + specialize (H0 s). cbn in *. destruct (x0 @ s), (y0 @ s). cbn in *.
+      red in H. destruct H. red in H, H1.
+      destruct H0. destruct H0.
+      split. split.
+      * intros. specialize (H0 _ H4). edestruct H0 as (? & ? & ?); clear H0.
+        exists x1. split; auto.
+      * intros. specialize (H3 _ H4). edestruct H3 as (? & ? & ?); clear H0.
+        exists x1. split; auto.
+      * auto.
+  - repeat intro. cbn in *. unfold eqmR_state in *.
+    specialize (H0 s).
+    destruct H0. destruct H0. cbn in *.
+    destruct (x0 @ s), (y0 @ s).
+    cbn in *.
+    split. split.
+    + intros. specialize (H0 _ H3). edestruct H0 as (? & ? & ?); clear H0.
+      exists x1. split; auto.
+    + intros. specialize (H2 _ H3). edestruct H2 as (? & ? & ?); clear H0.
+      exists x1. split; auto.
+    + auto.
   Qed.
 
   Lemma ret_stateT_P:
@@ -163,7 +218,8 @@ Section State.
 
   Lemma bind_stateT_P:
     forall (a b : typ) (f : a -=-> state S b) (sa : state S a),
-      Proper (equalE S ==> equalE (S × b)) (fun s : S => (f @ snd (sa @ s)) @ s).
+      Proper (equalE S ==> equalE (S × b))
+        (fun s : S => (f @ snd (sa @ s)) @ (fst (sa @ s))).
   Proof.
     intros a b f sa.
     repeat intro. rewrite H. reflexivity.
@@ -173,7 +229,7 @@ Section State.
     forall (a b : typ) (f : a -=-> state S b),
       Proper (equalE (state S a) ==> equalE (state S b))
               (fun sa : state S a =>
-                (-=->!) (fun s : S => (f @ snd (sa @ s)) @ s) (bind_stateT_P a b f sa)).
+                (-=->!) (fun s : S => (f @ snd (sa @ s)) @ (fst (sa @ s))) (bind_stateT_P a b f sa)).
   Proof.
     intros a b f.
     repeat intro. cbn. rewrite H, H0. split; reflexivity.
@@ -185,779 +241,296 @@ Section State.
   - intros. refine (-=->! (fun sa => _) (bind_stateT_P2 a b f)).
   Defined.
 
-  Instance EqmRMonadInverses_state `{inhabited S} : EqmRMonadInverses (state S).
-  constructor.
-  - intros. cbn in H. unfold eqmR_state in H.
-    cbn in H.
-    (* Need [inhabited S] here. *)
-    inversion inhabited0.
-    specialize (H X).
-    destruct H; auto.
-  - intros. cbn in *. unfold eqmR_state in *.
-    split.
-    + intros. specialize (H s).
-    (*   change (S ⊗ RB @ (((-=->!) (fun s : S => (k1 @ snd (ma @ s)) @ s) *)
-    (*                              (bind_stateT_P A B k1 ma)) @ s, *)
-    (*                     (-=->! (fun s : S => (k2 @ snd (ma @ s)) @ s) *)
-    (*                            (bind_stateT_P A B k2 ma)) @ s)) in H. *)
-    (*   destruct (S ⊗ RB). cbn in H. *)
-    (*   change (S ⊗ image (state S) ma @ (ma @ s, ma @ s)). *)
-    (*   destruct (ma @ s) eqn: H'. cbn in *. split. reflexivity. *)
-    (*   intros. *)
-    (*   unfold eqmR_state in EQ. *)
-    (*   change (forall s : S, S ⊗ R @ (ma @ s, ma @ s)) in EQ. *)
-    (*   specialize (EQ s). rewrite H' in EQ. cbn in EQ. destruct EQ. *)
-    (*   auto. *)
-    (* + intros. specialize (H s). *)
-    (*   change (S ⊗ RB @ ((-=->! (fun s : S => (k1 @ snd (ma @ s)) @ s) (bind_stateT_P A B k1 ma)) @ s, *)
-    (*                     (-=->! (fun s : S => (k2 @ snd (ma @ s)) @ s) *)
-    (*                            (bind_stateT_P A B k2 ma)) @ s)) in H. *)
-    (*   change (S ⊗ RB @ (k1 @ snd (ma @ s) @ s, *)
-    (*                     k2 @ snd (ma @ s) @ s)) in H. *)
-    (*   change (forall R : relationH A A, PER R -> *)
-    (*    (forall s : S, S ⊗ R @ (ma @ s, ma @ s)) -> R @ (a, a)) in H0. *)
-    (*   pose proof @prod_rel_PER. *)
-    (*   specialize (H1 S B S RB relationH_PER PH). *)
-    (*   change (S ⊗ RB @ (k1 @ a @ s, k2 @ a @ s)). *)
-      admit.
-  Admitted.
+  Definition state_prop {A : typ} (ma : state S A) :=
+    (fun a : A => exists s s', ma @ s == (s', a)).
+
+  Program Definition const_state {A : typ} (s : S) (a : A) : S -=-> (S × A) :=
+    -=->! (fun s => (s, a)) _.
+  Next Obligation.
+    repeat intro. split; cbn; eauto. reflexivity.
+  Qed.
+
+  Lemma mayRet_state {A:typ} (ma : state S A) (a : A) :
+    (exists s s' : S, (ma @ s) == (s', a)) <->
+    mayRet (state S) ma @ a.
+  Proof.
+    split. intro.
+    - cbn. intros. cbn in *. unfold eqmR_state in EQ.
+      cbn in *.
+      edestruct H as (? & ? & ?). clear H.
+      specialize (EQ x). destruct EQ. destruct H, H0.
+      specialize (H _ H3).
+      edestruct H as (? & ? & ?).
+      PER_reflexivityH.
+    - intros HM. do 6 red in HM.
+      intros.
+      epose ((-=->! (state_prop ma) _) : A -=-> prop_typ) as Q.
+      assert (eqmR (diagonal_prop Q) @ (ma, ma)).
+      { intro. cbn. split. split.
+        - intros.
+          unfold state_prop. exists a0.
+          split. split. intros.
+          exists s. destruct (ma @ s) eqn: Hma.
+          exists t. cbn in *. split; auto. reflexivity.
+          exists s. destruct (ma @ s) eqn: Hma.
+          cbn in *. exists t; split; auto. reflexivity.
+          auto.
+        - intros.
+          unfold state_prop. exists b.
+          split. split.
+          exists s. destruct (ma @ s) eqn: Hma.
+          exists t. cbn in *. split; auto. reflexivity.
+          exists s. destruct (ma @ s) eqn: Hma.
+          cbn in *. exists t; split; auto. reflexivity.
+          auto.
+        - reflexivity.
+      }
+      specialize (HM (diagonal_prop Q) (diagonal_prop_PER Q) H).
+      unfold diagonal_prop in HM. cbn in HM.
+      destruct HM as (HS & HS'); clear HS'. clear H.
+      unfold state_prop in HS.
+      edestruct HS as (? & ? & ?).
+      auto.
+      Unshelve.
+      repeat intro. unfold state_prop. cbn.
+      split.
+      setoid_rewrite H. auto. setoid_rewrite H. auto.
+  Qed.
+
+  Lemma mayRet_bind_state :
+    forall (A B : typ) (ma : state S A) (k : A -=-> state S B) (b : B),
+    mayRet (state S) (bind k @ ma) @ b ->
+    exists a : A, mayRet (state S) ma @ a /\ mayRet (state S) (k @ a) @ b.
+  Proof.
+    intros.
+    setoid_rewrite <- mayRet_state. setoid_rewrite <- mayRet_state in H.
+    edestruct H as (? & ? & ?); clear H.
+    cbn in H0. destruct H0. destruct (ma @ x) eqn : Hma. cbn in *.
+    exists t0. split.
+    - exists x. rewrite Hma. cbn. exists t. split; reflexivity.
+    - exists t, x0. split; auto.
+  Qed.
+
+  Opaque mayRet.
 
   Lemma eqmR_bind_ProperH_state :
-    forall (s : S) (A1 A2 B1 B2 : typ) (RA : relationH A1 A2) (RB : relationH B1 B2)
+    forall (A1 A2 B1 B2 : typ) (RA : relationH A1 A2) (RB : relationH B1 B2)
       (ma1 : state S A1) (ma2 : state S A2) (kb1 : A1 -=-> state S B1)
       (kb2 : A2 -=-> state S B2),
     eqmR RA @ (ma1, ma2) ->
-    (forall (a1 : A1) (a2 : A2),
+    (forall a1 : A1,
     mayRet (state S) ma1 @ a1 ->
-    mayRet (state S) ma2 @ a2 -> RA @ (a1, a2) -> eqmR RB @ (kb1 @ a1, kb2 @ a2)) ->
+    forall a2 : A2, RA @ (a1, a2) -> eqmR RB @ (kb1 @ a1, kb2 @ a2)) ->
+    (forall a2 : A2,
+    mayRet (state S) ma2 @ a2 ->
+    forall a1 : A1, RA @ (a1, a2) -> eqmR RB @ (kb1 @ a1, kb2 @ a2)) ->
     eqmR RB @ (bind kb1 @ ma1, bind kb2 @ ma2).
   Proof.
     intros.
+    cbn in *. unfold eqmR_state in *. cbn in *. intro.
+    specialize (H s).
+    destruct H. destruct H.
+    destruct (ma1 @ s) eqn: Hma1.
+    destruct (ma2 @ s) eqn: Hma2.
+    cbn in *.
+    specialize (H t0 equal_typ).
+    specialize (H3 t2 equal_typ).
+    edestruct H as (? & ? & ?); clear H.
+    edestruct H3 as (? & ? & ?); clear H3.
+    specialize (H0 t0). specialize (H1 t2).
+    assert (mayRet (state S) ma1 @ t0). {
+      rewrite <- mayRet_state. exists s, t. rewrite Hma1. reflexivity.
+    }
+    assert (mayRet (state S) ma2 @ t2). {
+      rewrite <- mayRet_state. exists s, t1. rewrite Hma2. reflexivity.
+    }
+    specialize (H0 H3 _ H4 t1). specialize (H1 H7 x0 H t1).
+    setoid_rewrite H6. setoid_rewrite H2. auto.
+  Qed.
 
-  Admitted.
+  Lemma image_eqmR_state :
+    forall (A : typ) (ma : state S A), eqmR (image (state S) ma) @ (ma, ma).
+  Proof.
+    intros. cbn. unfold eqmR_state. intros. cbn.
+    destruct (ma @ s) eqn: Hma.
+    cbn in *. split. split.
+    - intros. exists a. split. intros. unfold eqmR_state in EQ. cbn in *.
+      specialize (EQ s). setoid_rewrite Hma in EQ.
+      cbn in EQ. destruct EQ. destruct H0.
+      specialize (H0 a H).
+      edestruct H0 as (? & ? & ?); clear H0.
+      PER_reflexivityH. auto.
+    - intros. exists b. split. intros. unfold eqmR_state in EQ. cbn in *.
+      specialize (EQ s). setoid_rewrite Hma in EQ.
+      cbn in EQ. destruct EQ. destruct H0.
+      specialize (H0 b H).
+      edestruct H0 as (? & ? & ?); clear H0.
+      PER_reflexivityH. auto.
+    - reflexivity.
+  Qed.
+
+  Lemma eqmR_mayRet_l :
+    forall (A1 A2 : typ) (RA : relationH A1 A2) (ma1 : state S A1)
+      (ma2 : state S A2),
+    eqmR RA @ (ma1, ma2) ->
+    forall a1 : A1,
+    mayRet (state S) ma1 @ a1 ->
+    exists a2 : A2, RA @ (a1, a2) /\ mayRet (state S) ma2 @ a2.
+  Proof.
+    intros.
+    rewrite <- mayRet_state in H0. edestruct H0 as (? & ? & ?); clear H0.
+    cbn in *. destruct (ma1 @ x) eqn: Hma. cbn in *.
+    destruct H1. unfold eqmR_state in H. cbn in H.
+    specialize (H x). setoid_rewrite Hma in H.
+    cbn in *. setoid_rewrite <- mayRet_state.
+    destruct (ma2 @ x) eqn: Hma2. cbn in *.
+    destruct H. destruct H.
+    specialize (H _ H1). edestruct H as (? & ? & ?); clear H.
+    specialize (H3 _ H5). edestruct H3 as (? & ? & ?); clear H3.
+    exists x1. split. auto. exists x, t1. split. rewrite Hma2. reflexivity.
+    rewrite Hma2. auto.
+  Qed.
+
+  Lemma eqmR_mayRet_r :
+    forall (A1 A2 : typ) (RA : relationH A1 A2) (ma1 : state S A1)
+      (ma2 : state S A2),
+    eqmR RA @ (ma1, ma2) ->
+    forall a2 : A2,
+    mayRet (state S) ma2 @ a2 ->
+    exists a1 : A1, RA @ (a1, a2) /\ mayRet (state S) ma1 @ a1.
+  Proof.
+    intros.
+    rewrite <- mayRet_state in H0. edestruct H0 as (? & ? & ?); clear H0.
+    cbn in *. destruct (ma1 @ x) eqn: Hma. cbn in *.
+    destruct H1. unfold eqmR_state in H. cbn in H.
+    specialize (H x). setoid_rewrite Hma in H.
+    cbn in *. setoid_rewrite <- mayRet_state.
+    destruct (ma2 @ x) eqn: Hma2. cbn in *.
+    destruct H. destruct H.
+    specialize (H3 _ H1). edestruct H3 as (? & ? & ?); clear H3.
+    specialize (H _ H5). edestruct H as (? & ? & ?); clear H.
+    exists x1. split. auto. exists x, t. split. rewrite Hma. reflexivity.
+    rewrite Hma. auto.
+  Qed.
+
+  Lemma eqmR_ret_state :
+    forall (A1 A2 : typ) (RA : relationH A1 A2) (a1 : A1) (a2 : A2),
+    RA @ (a1, a2) -> eqmR (m := state S) RA @ (ret @ a1, ret @ a2).
+  Proof.
+    intros. cbn. unfold eqmR_state. cbn. intros.
+    split. split.
+    - intros. setoid_rewrite <- H0. exists a2. split; intuition.
+    - intros. setoid_rewrite <- H0. exists a1. split; intuition.
+    - reflexivity.
+  Qed.
+
+  Lemma eqmR_bind_ret_l_state:
+    forall (A B : typ) (f : A -=-> state S B) (a : A), bind f @ (ret @ a) == f @ a.
+  Proof.
+    intros. repeat red. cbn. intros. split. rewrite H. reflexivity.
+    rewrite H. reflexivity.
+  Qed.
+
+  Lemma eqmR_bind_ret_r_state:
+    forall A : typ, typ -> forall ma : state S A, bind ret @ ma == ma.
+  Proof.
+    repeat intro. cbn. rewrite H. split; reflexivity.
+  Qed.
+
+  Lemma eqmR_bind_bind_state:
+    forall (A B C : typ) (ma : state S A) (f : A -=-> state S B)
+      (g : B -=-> state S C), (bind f >>> bind g) @ ma ==
+                              bind (f >>> bind g) @ ma.
+  Proof.
+    repeat intro. cbn.
+    assert (exists s1 a1, ma @ x == (s1, a1)). {
+      destruct (ma @ x) eqn: Hma.
+      exists t, t0. reflexivity.
+    }
+    assert (exists s1 a1, ma @ y == (s1, a1)). {
+      destruct (ma @ y) eqn: Hma.
+      exists t, t0. reflexivity.
+    }
+    edestruct H0 as (? & ? & ?).
+    edestruct H1 as (? & ? & ?).
+    clear H0; clear H1.
+    rewrite H2. cbn.
+    change (
+      fst ((g @ snd ((f @ x1) @ x0)) @ fst ((f @ x1) @ x0)) ==
+      fst
+        ((g @ snd (f @ (snd (ma @ y)) @ fst (ma @ y))) @
+        fst (f @ (snd (ma @ y)) @ fst (ma @ y))) /\
+      snd ((g @ snd ((f @ x1) @ x0)) @ fst ((f @ x1) @ x0)) ==
+      snd
+        ((g @ snd (f @ (snd (ma @ y)) @ fst (ma @ y))) @
+        fst (f @ (snd (ma @ y)) @ fst (ma @ y)))).
+    rewrite H3. cbn. rewrite <- H in H3. rewrite H2 in H3.
+    destruct H3. cbn in *. rewrite H0. rewrite H1. split; reflexivity.
+  Qed.
 
   Instance EqmRMonad_state : EqmRMonad (state S).
   constructor.
-  - intros. cbn. unfold eqmR_state. intro.
-    change (S ⊗ image (state S) ma @ (ma @ s, ma @ s)).
-    destruct (ma @ s) eqn: H'. cbn. split. reflexivity.
-    intros. unfold eqmR_state in EQ.
-    change (forall s, S ⊗ R @ (ma @ s, ma @ s)) in EQ.
-    specialize (EQ s). rewrite H' in EQ. cbn in EQ. destruct EQ. auto.
-  - intros. cbn in *.
-    unfold eqmR_state in H.
-    eexists ?[a]. split.
-    + intros.
-      change (forall s, S ⊗ R @ (ma @ s, ma @ s)) in EQ.
-      assert (inhabited S). admit. (* Need to assume [inhabited S]. *)
-      admit.
-    + intros. apply H; auto. intros. admit.
-      (* Trying to play with alternative.. *)
-  - intros. admit.
-  - admit.
-  - admit.
-  -  admit. 
-  Admitted.
-
-  (* Instance EqmRMonad_state : EqmRMonad (state S). *)
-  (* constructor. *)
-  (* Admitted. *)
-
-End State.
-
-Section StateT.
-  Variable m : typ -> typ.
-  Variable S : typ.
-  Context {Mm : Monad typ_proper m}.
-  Context {EqmRm : EqmR m}.
-  Context {EqmROKm : EqmR_OK m}.
-  Context {EqmRInv : EqmRMonadInverses m}.
-  Context {ML : EqmRMonad m}.
-
-  (* Ported from Basics, the monad definitions on Basics should all change with
-     typ. *)
-  Definition stateT (s : typ) (m : typ -> typ) (a : typ) : typ :=
-    s ~~> m (prod_typ s a).
-
-  Global Instance EqmR_stateT : EqmR (stateT S m).
-  econstructor. Unshelve. 2 : {
-    refine (
-        fun A B (R : relationH A B) =>
-        -=->! (fun (p : stateT S m A × stateT S m B) =>
-                   forall (s : S), eqmR (S ⊗ R) @ ((fst p) @ s, (snd p) @ s)) _).
-    repeat intro. setoid_rewrite H. reflexivity.
-  }
-  repeat intro; split; repeat intro; cbn in *.
-  - rewrite H0.
-    eapply eqmR_equal.
-    eapply eqmR_Proper_mono; eauto.
-    repeat red. intros. destruct x1, y1. cbn in *. apply H1.
-  - eapply eqmR_Proper_mono; eauto.
-    2 : { eapply eqmR_equal in H. 2 : reflexivity. apply H. }
-    apply prod_rel_eq.
-  Defined.
-
-  (* Lemma eqmR_rel_prod : forall {A B : typ} *)
-  (*                       (R : relationH A B) *)
-  (*                       (x : A) (y : B) (s : S), *)
-  (*   R @ (x, y) -> *)
-  (*   eqmR (m := stateT S m) (S ⊗ R) @ (ret @ ((s, x),(s, y))). *)
-
-  Global Instance EqmR_OK_stateT : EqmR_OK (stateT S m).
-  Proof.
-    split; unfold eqmR, EqmR_stateT; intros.
-    - red. cbn. intros.
-      epose proof @prod_rel_refl.
-      rewrite ReflexiveH_Reflexive in H.
-      specialize (H0 _ _ S _ _ H).
-      eapply eqmR_transport_refl in H0; eauto.
-    - red. cbn. intros.
-      epose proof @prod_rel_sym.
-      apply SymmetricH_Symmetric in H.
-      specialize (H1 S A S R _ H).
-      eapply eqmR_transport_symm in H0; eauto.
-      2 : { apply SymmetricH_Symmetric; eauto. }
-      cbn in H0. apply H0.
-    - cbn . intros!. cbn in *.
-      apply TransitiveH_Transitive in H.
-      epose proof @prod_rel_trans.
-      specialize (H3 S A S R _ H).
-      pose proof @eqmR_transport_trans.
-      apply TransitiveH_Transitive in H3.
-      specialize (H4 m _ _ _ _ H3).
-      red in H4. red in H2.
-      specialize (H4 (fst p @ s, snd p @ s) (fst q @ s, snd q @ s)).
-      specialize (H4 (H0 s) (H1 s)).
-      cbn in H4. apply H4.
-      apply H2. reflexivity.
-    - red; cbn; repeat intro. cbn in *.
-      specialize (H s). specialize (H0 s).
-      eapply eqmR_Proper; eauto.
-      rewrite <- (eq_id_r S).
-      rewrite prod_compose. reflexivity.
-      eapply eqmR_rel_trans; auto.
-      + apply H.
-      + apply H0.
-    - split; intros smb sma Heq s.
-      + specialize (Heq s).
-        cbn in *.
-        apply eqmR_lift_transpose; eauto.
-        eapply eqmR_Proper; eauto.
-        rewrite transpose_prod.
-        rewrite transpose_sym_eq_rel; eauto. reflexivity.
-        typeclasses eauto.
-      + unfold transpose in Heq. specialize (Heq s).
-        eapply eqmR_Proper; eauto.
-        rewrite <- transpose_sym_eq_rel; auto.
-        rewrite <- transpose_prod.
-        reflexivity. typeclasses eauto.
-        cbn in *. apply eqmR_lift_transpose; auto.
-    - repeat intro. cbn in *. split.
-      +  repeat intro. cbn.
-          specialize (H0 s). cbn in *.
-          eapply eqmR_Proper; eauto.
-          rewrite H. reflexivity.
-      + repeat intro. cbn.
-        specialize (H0 s). cbn in *.
-        eapply eqmR_Proper; eauto.
-        rewrite H. reflexivity.
-    - repeat red. repeat intro. specialize (H0 s).
-      eapply (eqmR_Proper_mono) in H0; eauto.
-      apply prod_rel_monotone. intuition. eauto.
+  - apply image_eqmR_state.
+  - apply mayRet_bind_state.
+  - apply eqmR_mayRet_l.
+  - apply eqmR_mayRet_r.
+  - apply eqmR_ret_state.
+  - apply eqmR_bind_ProperH_state.
+  - apply eqmR_bind_ret_l_state.
+  - apply eqmR_bind_ret_r_state.
+  - apply eqmR_bind_bind_state.
   Qed.
 
-  (* Making properness proofs opaque, so it's doesn't do the ugly unfolding in
-   proof contexts *)
-  Lemma Proper_ret :
-    forall (a : typ) (x : a),
-      Proper (equalE S ==> equalE (m (S × a))) (fun s : S => ret @ (s, x)).
-  Proof.
-    repeat intro. rewrite H. reflexivity.
-  Qed.
-
-  Lemma Proper_ret_2 :
-    forall (a : typ),
-      Proper (equalE a ==> equalE (S ~~> m (S × a)))
-         (fun x : a => (-=->!) (fun s : S => ret @ (s, x)) (Proper_ret a x)).
-  Proof.
-    repeat intro. cbn. rewrite H0, H. reflexivity.
-  Qed.
-
-  Lemma Proper_bind:
-    forall (a b : typ) (f : a -=-> stateT S m b),
-      S ~~> m (S × a) ->
-      S ->
-      Proper (equalE (S × a) ==> equalE (m (S × b)))
-              (fun y : S * a => uncurry f @ (snd y, fst y)).
+  Lemma eqmR_bind_inv_state:
+    forall (A B : typ) (RB : relationH B B),
+    SymmetricH RB ->
+    TransitiveH RB ->
+    forall (ma : state S A) (k : A -=-> state S B) (b : B),
+    mayRet (state S) (bind k @ ma) @ b ->
+    eqmR (image (state S) ma) @ (ma, ma) /\
+    (exists a : A, mayRet (state S) ma @ a ->
+              mayRet (state S) (k @ a) @ b).
   Proof.
     repeat intro.
-    destruct x, y. cbn.
-    destruct H. cbn in *. rewrite H, H0. reflexivity.
-  Defined.
-
-  Lemma Proper_bind_2:
-    forall (a b : typ) (f : a -=-> stateT S m b) (k : S ~~> m (S × a)),
-      Proper (equalE S ==> equalE (m (S × b)))
-          (fun x : S =>
-            let X :=
-                (-=->!) (fun y : S * a => uncurry f @ (snd y, fst y))
-                        (Proper_bind a b f k x) in
-            @bind typ typ_proper m Mm (S × a) (S × b) X @ (k @ x)).
-  Proof.
-    repeat intro. unfold uncurry. cbn. unfold Proper_bind.
-    rewrite H.
-    reflexivity.
+    split; [ split ; [ split | ] | ].
+    - cbn. rewrite <- mayRet_state in H1.
+      cbn in *. intros. exists a. split; auto. intros.
+      unfold eqmR_state in EQ. cbn in EQ.
+      specialize (EQ s). destruct EQ. destruct H3.
+      specialize (H3 a H2).
+      edestruct H3 as (? & ? & ?).
+      PER_reflexivityH.
+    - rewrite <- mayRet_state in H1.
+      edestruct H1 as (? & ? & ?); clear H1.
+      cbn. intros. exists b0. split; auto. intros.
+      unfold eqmR_state in EQ. cbn in EQ.
+      specialize (EQ s). destruct EQ. destruct H3.
+      specialize (H5 _ H1).
+      edestruct H5 as (? & ? & ?).
+      PER_reflexivityH.
+    - cbn. reflexivity.
+    - cbn; intros.
+      rewrite <- mayRet_state in H1. edestruct H1 as (? & ? & ?); clear H1.
+      cbn in H2. destruct H2.
+      destruct (ma @ x) eqn: H'. cbn in *.
+      exists t0. intros.
+      rewrite <- mayRet_state in H3. edestruct H3 as (? & ? & ?); clear H3.
+      rewrite <- mayRet_state.
+      exists t. exists x0. destruct ((k @ t0) @ t). cbn in *. split; auto.
   Qed.
 
-  Lemma Proper_bind_3:
-    forall (a b : typ) (f : a -=-> stateT S m b),
-      @Proper (S ~~> m (S × a) -> S ~~> m (S × b))
-              (equalE (S ~~> m (S × a)) ==> equalE (S ~~> m (S × b)))
-              (fun k : S ~~> m (S × a) =>
-                  (-=->!)
-                    (fun x : S =>
-                      let X :=
-                          (-=->!)
-                            (fun y : S * a =>
-                                @uncurry a S (m (S × b)) f @ (@snd S a y, @fst S a y))
-                            (Proper_bind a b f k x) in
-                      @bind typ typ_proper m Mm (S × a) (S × b) X @ (k @ x))
-                    (Proper_bind_2 a b f k)).
-  Proof.
-    intros a b f. unfold Proper_bind.
-    repeat intro. unfold uncurry. cbn. rewrite H.
-    rewrite H0. reflexivity.
-  Qed.
-
-  Set Transparent Obligations.
-  (* ret and bind definition for stateT. *)
-  Program Instance stateT_Monad : Monad typ_proper (stateT S m).
-  Next Obligation.
-  intros. unfold stateT. refine (-=->! (fun x => _) _).
-  Unshelve. 2 : {
-      refine (-=->! (fun s => ret @ (s, x)) _). apply Proper_ret.
-  } apply Proper_ret_2.
-  Defined.
-  Next Obligation.
-  unfold stateT. intros.
-  refine (-=->! (fun k => _) _).
-  Unshelve. 2 : {
-    refine (-=->! (fun x => _) _).
-    Unshelve. 2 : {
-      assert ((S × a) -=-> m (S × b)). {
-        refine (-=->! (fun y => uncurry f @ (snd y, fst y)) _).
-        apply Proper_bind; eauto.
-      }
-      exact ((bind X) @ (k @ x)).
-    }
-      apply Proper_bind_2; eauto.
-  }
-  apply Proper_bind_3; eauto.
-  Defined.
-
-  Lemma relate_state_proper:
-    forall (A1 : typ) (R : relationH A1 A1),
-      Proper (equalE ((S × A1) × (S × A1)) ==> equalE prop_typ)
-             (fun p : S * A1 * (S * A1) =>
-                fst (fst p) == fst (snd p) /\ R @ (snd (fst p), snd (snd p))).
-  Proof.
-    repeat intro. destruct x, y. destruct t, t0, t1, t2. cbn.
-    split; intro.
-    destruct H. cbn in H, H1. destruct H, H0, H1.
-    split. rewrite <- H. rewrite <- H1. auto.
-    rewrite <- H2. rewrite <- H4. auto.
-    destruct H. cbn in H, H1. destruct H, H0, H1.
-    split. rewrite H. rewrite H1. auto.
-    rewrite H2. rewrite H4. auto.
-  Qed.
-
-  Program Definition relate_state {A1 : typ} (R : relationH A1 A1) : relationH (S × A1) (S × A1).
-  refine (-=->! (fun (p : (S * A1) * (S * A1)) => fst (fst p) == fst (snd p) /\ R @ (snd (fst p), snd (snd p))) _).
-  apply relate_state_proper; auto.
-  Defined.
-
-
-  Lemma relate_state_Symmetric {A1 : typ} (R : relationH A1 A1)
-        (RH: SymmetricH R): SymmetricH (relate_state R).
-  Proof.
-    repeat intro. cbn. destruct p. destruct t, t0. destruct H.
-    cbn in *. split. symmetry; auto. apply SymmetricH_Symmetric in RH.
-    apply RH. apply H0.
-  Qed.
-
-  Lemma relate_state_Transitive {A1 : typ} (R : relationH A1 A1)
-        (RH: TransitiveH R) : TransitiveH (relate_state R).
-  Proof.
-    repeat intro. cbn. destruct p. destruct t, t0. destruct H.
-    cbn in *. destruct H0, H1. destruct q, p, p0. cbn in *. split.
-    rewrite <- H0. rewrite <- H1. apply H.
-    apply TransitiveH_Transitive in RH.
-    eapply RH. apply H2. rewrite H4. apply H3.
-  Qed.
-
-  Program Definition snd_prj {B} (R: relationH (S × B) (S × B)) (t : S): relationH B B := (-=->! (fun p => R @ ((t, fst p),(t, snd p))) _).
-  Next Obligation.
-    repeat intro. destruct x, y. cbn in H. destruct H; cbn.
-    split. intros. rewrite <- H; rewrite <- H0. auto.
-    intros. rewrite H, H0. auto.
-  Defined.
-
-  Lemma stateT_inv_equal {A1 A2 : typ} :
-    forall (RA : relationH A1 A2) (sma1 : stateT S m A1)
-      (sma2 : stateT S m A2),
-      eqmR RA @ (sma1, sma2) ->
-      forall (ma1 : m A1), exists (ma2 : m A2), eqmR RA @ (ma1, ma2).
+  Context `{inhabited S}.
+  Instance EqmRMonadInverses_state : EqmRMonadInverses (state S).
+  constructor.
+  - repeat intro.
+    cbn in H. unfold eqmR_state in H. cbn in H.
+    inversion inhabited0. specialize (H X).
+    destruct H. destruct H.
+    specialize (H a1 equal_typ). edestruct H as (? & ? & ?); clear H.
+    specialize (H1 a2 equal_typ). edestruct H1 as (? & ? & ?); clear H1.
+    rewrite H3. auto.
+  - admit.
+  - apply eqmR_bind_inv_state.
   Admitted.
 
-
-  Lemma stateT_image:
-    forall (A : typ) (ma : stateT S m A), eqmR (image (stateT S m) ma) @ (ma, ma).
-  Admitted.
-
-  Definition curry_swap' {A B} (k : A -=-> (S ~~> m (S × B))) : (S × A) -> m (S × B) := fun p => k @ (snd p) @ (fst p).
-
-  Lemma curry_swap_Proper:
-    forall {A B}
-      (k : A -=-> (S ~~> m (S × B))),
-  Proper (equalE (S × A) ==> equalE (m (S × B))) (curry_swap' k).
-  Proof.
-    repeat intro. cbn. destruct x, y. cbn in *. destruct H.
-    unfold curry_swap'.
-    rewrite H, H0. reflexivity .
-  Qed.
-
-  Definition curry_swap {A B} (k : A -=-> (S ~~> m (S × B))) : (S × A) -=-> m (S × B) := (-=->! (curry_swap' k) (curry_swap_Proper k)).
-
-
-  (* Lemma mayRet_stateT {A:typ} (ma : stateT S m A) (a : A) : *)
-  (*   forall s, (ma @ s) <-> mayRet (stateT S m) ma @ a. *)
-
-  Lemma mayRet_stateT_bind :
-    forall {A B : typ} (ma : stateT S m A)
-      (k : A -=-> stateT S m B) (b : B),
-      mayRet (stateT S m) (bind k @ ma) @ b ->
-      exists (ma' : m A) (k' : A -=-> m B),
-      mayRet m (bind k' @ ma') @ b.
-  Proof.
-    intros. Admitted.
-
-  (* Lemma stateT_image_refl {A : typ} : *)
-  (*   forall (x : m A) (ma' : m A), *)
-  (*   eqmR (image m ma') @ (x, x) -> eqmR (image (stateT S m)) @ (x, x). *)
-  (* Proof. *)
-  (* Admitted. *)
-
-  Lemma eqmR_prod_inv {A : typ}:
-    forall (ma' : m A) (ma : stateT S m A) (s : S) (R : relationH A A),
-      eqmR R @ (ma', ma') ->
-      eqmR (S ⊗ R) @ (ma @ s, ma @ s).
-  Admitted.
-
-  Lemma stateT_mayRet_bind :
-    forall (A B : typ) (ma : stateT S m A) (k : A -=-> stateT S m B) (b : B),
-    mayRet (stateT S m) (bind k @ ma) @ b ->
-    exists a : A, mayRet (stateT S m) ma @ a /\ mayRet (stateT S m) (k @ a) @ b.
-  Proof.
-    intros.
-    pose proof mayRet_bind as HMB.
-    specialize (HMB m _ _ _).
-    pose proof (mayRet_stateT_bind _ _ _ H) as HBind.
-    edestruct HBind as (ma' & k' & bind'); clear HBind.
-    specialize (HMB A B _ _ _ bind').
-    edestruct HMB as (a & prefix & cont); clear HMB.
-    exists a. split.
-    - eapply prefix. eapply image_PER.
-      eapply eqmR_Proper; eauto.
-      + Unshelve.
-        2 : { exact (image m ma'). }
-        split; repeat intro.
-        * apply H0; eauto. intro. cbn.
-          remember (ma @ s).
-          admit.
-        * apply H0; eauto. cbn in EQ. admit.
-      + admit. 
-    - pose proof mayRet_bind as HMB.
-      specialize (HMB m _ _ _).
-      pose proof (mayRet_stateT_bind _ _ _ H) as HBind.
-      edestruct HBind as (? & ? & ?).
-      specialize (HMB A B _ _ _ H0).
-      edestruct HMB.
-      destruct H1.
-      intro. cbn. intros. apply H2. 
-    (*   intro. intro.  *)
-    (*   edestruct HMB as (? & ? & ?). *)
-
-    (*   repeat intro.  *)
-    (*   repeat red in H. cbn in H. *)
-    (*   cbn.  *)
-    (*   unfold stateT in *. *)
-    (*   edestruct HMB; eauto. *)
-    (*   + repeat red. intros. apply H; eauto. repeat intro. cbn. *)
-    (*     eapply eqmR_bind_ProperH; eauto. *)
-    (*     * eapply eqmR_equal. cbn. reflexivity. *)
-    (*     * cbn. intros. destruct a1, a2. cbn in *. destruct H2. *)
-    (*       rewrite H2, H3. *)
-
-    (*       eapply eqmR_Proper_mono; eauto. *)
-    (*       eapply image_least. eapply prod_rel_PER; auto. *)
-    (*       eapply relationH_PER. *)
-    (*       -- admit. *)
-    (*       -- eapply image_eqmR; eauto. *)
-    (*   + destruct H0. *)
-    (*     apply H0.  *)
-    (*     repeat intro. *)
-
-    (* - cbn. intros. cbn in H. apply H; eauto. intros. *)
-    (*   eapply eqmR_bind_ProperH; eauto. *)
-    (*   + eapply eqmR_equal. cbn. reflexivity. *)
-    (*   + pose proof mayRet_bind. specialize (EQ s). intros. cbn. *)
-    (*     destruct a1, a2. cbn in *. *)
-    (*     destruct H3. rewrite H3. rewrite H4. *)
-
-    (*     eapply eqmR_transport_refl; eauto. *)
-    (*     red. intro. destruct a. cbn. split. reflexivity. *)
-        (* reflexivity.  *)
-  Admitted.
-
-  Lemma stateT_eqmR_mayRet_l :
-    forall (A1 A2 : typ) (ma1 : stateT S m A1) (ma2 : stateT S m A2)
-      (RA : relationH A1 A2),
-    eqmR RA @ (ma1, ma2) ->
-    forall a1 : A1,
-    mayRet (stateT S m) ma1 @ a1 ->
-    exists a2 : A2, RA @ (a1, a2) /\ mayRet (stateT S m) ma2 @ a2.
-  Proof.
-    intros*. intros EQ' a1 HMR.
-    pose proof eqmR_mayRet_l as H.
-    specialize (H m _ _ _ _ _ RA).
-    pose proof @stateT_inv_equal as HI.
-    specialize (HI _ _ RA ma1 ma2 EQ').
-    edestruct HI.
-    edestruct H.
-    - cbn in EQ'. apply H0.
-    - apply HMR.
-      + eapply image_PER.
-      + cbn. intros. clear H0.
-        clear HI.
-        eapply eqmR_transport_refl; eauto.
-        repeat intro. cbn. destruct a. split.
-        reflexivity. intros.
-        eapply eqmR_ret_inv in EQ.
-        admit. auto.
-    - exists x0. destruct H1. split; auto. apply H2.
-      eapply image_PER.
-  Admitted.
-
-  Lemma stateT_eqmR_mayRet_r :
-    forall (A1 A2 : typ) (ma1 : stateT S m A1) (ma2 : stateT S m A2)
-      (RA : relationH A1 A2),
-    eqmR RA @ (ma1, ma2) ->
-    forall a2 : A2,
-    mayRet (stateT S m) ma2 @ a2 ->
-    exists a1 : A1, RA @ (a1, a2) /\ mayRet (stateT S m) ma1 @ a1.
-  Proof.
-  Admitted.
-
-  Instance EqmRMonad_stateT : @EqmRMonad (stateT S m) _ _.
-  Proof.
-    constructor.
-    - admit.
-    - apply stateT_mayRet_bind.
-    -
-    (*   apply stateT_eqmR_mayRet_l. *)
-    (* - apply stateT_eqmR_mayRet_r. *)
-  Admitted.
-
-(*   Context {Im: Iter (Kleisli m) sum}. *)
-(*   Context {Cm: Iterative (Kleisli m) sum}. *)
-
-(*   Definition iso {a b:Type} (sab : S * (a + b)) : (S * a) + (S * b) := *)
-(*     match sab with *)
-(*     | (s, inl x) => inl (s, x) *)
-(*     | (s, inr y) => inr (s, y) *)
-(*     end. *)
-
-(*   Definition iso_inv {a b:Type} (sab : (S * a) + (S * b)) : S * (a + b) := *)
-(*     match sab with *)
-(*     | inl (s, a) => (s, inl a) *)
-(*     | inr (s, b) => (s, inr b) *)
-(*     end. *)
-
-(*   Definition internalize {a b:Type} (f : Kleisli (stateT S m) a b) : Kleisli m (S * a) (S * b) := *)
-(*     fun (sa : S * a) => f (snd sa) (fst sa). *)
-
-(*   Lemma internalize_eq {a b:Type} (f g : Kleisli (stateT S m) a b) : *)
-(*     eq2 f g <-> eq2 (internalize f) (internalize g). *)
-(*   Proof. *)
-(*     split. *)
-(*     - intros. *)
-(*       repeat red. destruct a0. *)
-(*       unfold internalize. cbn.  specialize (H a0 s). unfold eqmR in H. *)
-(*       rewrite prod_rel_eq in H. apply H. *)
-(*     - intros. *)
-(*       repeat red. intros. *)
-(*       unfold internalize in H. *)
-(*       specialize (H (s, a0)). *)
-(*       rewrite prod_rel_eq. *)
-(*       apply H. *)
-(*   Qed. *)
-
-(*   Lemma internalize_cat {a b c} (f : Kleisli (stateT S m) a b) (g : Kleisli (stateT S m) b c) : *)
-(*     (internalize (f >>> g)) ⩯ ((internalize f) >>> (internalize g)). *)
-(*   Proof. *)
-(*     repeat red. *)
-(*     destruct a0. *)
-(*     cbn. *)
-(*     unfold internalize. *)
-(*     unfold cat, Cat_Kleisli. *)
-(*     cbn. *)
-(*     reflexivity. *)
-(*   Qed. *)
-
-(*   Lemma internalize_pure {a b c} (f : Kleisli (stateT S m) a b) (g : S * b -> S * c) : *)
-(*     internalize f >>> pure g   ⩯   (internalize (f >>> (fun b s => ret (g (s,b))))). *)
-(*   Proof. *)
-(*     repeat red. *)
-(*     destruct a0. *)
-(*     unfold internalize, cat, Cat_Kleisli. cbn. *)
-(*     apply Proper_bind; auto. *)
-(*     - reflexivity. *)
-(*     - repeat red. *)
-(*       destruct a1. *)
-(*       unfold pure. reflexivity. *)
-(*   Qed. *)
-
-(*   Global Instance Iter_stateT : Iter (Kleisli (stateT S m)) sum. *)
-(*   Proof. *)
-(*     exact *)
-(*       (fun (a b : Type) (f : a -> S -> m (S * (a + b))) (x:a) (s:S) => *)
-(*         iter ((internalize f) >>> (pure iso)) (s, x)). *)
-(*   Defined. *)
-
-(*   Global Instance Proper_Iter_stateT : forall a b, @Proper (Kleisli (stateT S m) a (a + b) -> (Kleisli (stateT S m) a b)) (eq2 ==> eq2) iter. *)
-(*   Proof. *)
-(*     destruct Cm. *)
-(*     repeat red. *)
-(*     intros a b x y H a0 s. *)
-(*     rewrite prod_rel_eq. *)
-(*     apply iterative_proper_iter. *)
-(*     repeat red. *)
-(*     destruct a1. *)
-(*     cbn. *)
-(*     apply Proper_bind. *)
-(*     - unfold internalize. cbn. (specialize (H a1 s0)). rewrite prod_rel_eq in H. apply H. *)
-(*     - repeat red. destruct a2 as [s' [x1|y1]]; reflexivity. *)
-(*   Qed. *)
-
-(*   Global Instance IterUnfold_stateT : IterUnfold (Kleisli (stateT S m)) sum. *)
-(*   Proof. *)
-(*   destruct Cm. *)
-(*   unfold IterUnfold. *)
-(*   intros a b f. *)
-(*   repeat red. *)
-(*   intros a0 s. *)
-(*   unfold cat, Cat_Kleisli. *)
-(*   unfold iter, Iter_stateT. *)
-(*   rewrite iterative_unfold.  (* SAZ: why isn't iter_unfold exposed here? *) *)
-(*   unfold cat, Cat_Kleisli. *)
-(*   simpl. *)
-(*   rewrite bind_bind. rewrite prod_rel_eq. *)
-(*   apply Proper_bind. *)
-(*   + reflexivity. *)
-(*   + repeat red. destruct a1 as [s' [x | y]]; simpl. *)
-(*     * unfold pure. rewrite bind_ret_l. *)
-(*       reflexivity. *)
-(*     * unfold pure. rewrite bind_ret_l. *)
-(*       reflexivity. *)
-(*   Qed. *)
-
-(*   Global Instance IterNatural_stateT : IterNatural (Kleisli (stateT S m)) sum. *)
-(*   Proof. *)
-(*     destruct Cm. *)
-(*     unfold IterNatural. *)
-(*     intros a b c f g. *)
-(*     repeat red. *)
-(*     intros a0 s. *)
-(*     setoid_rewrite iterative_natural. rewrite prod_rel_eq. *)
-(*     apply iterative_proper_iter. *)
-(*     repeat red. *)
-(*     destruct a1. *)
-(*     unfold cat, Cat_Kleisli. *)
-(*     cbn. *)
-(*     rewrite! bind_bind. *)
-(*     apply Proper_bind. *)
-(*     - reflexivity. *)
-(*     - repeat red. destruct a2 as [s' [x | y]]; simpl. *)
-(*       + unfold pure. rewrite bind_ret_l. *)
-(*         cbn. unfold cat, Cat_Kleisli. cbn. *)
-(*         rewrite bind_bind. *)
-(*         rewrite bind_ret_l. *)
-(*         rewrite bind_ret_l. *)
-(*         cbn. *)
-(*         unfold id_, Id_Kleisli. unfold pure. rewrite bind_ret_l. reflexivity. *)
-(*       + unfold pure. rewrite bind_ret_l. *)
-(*         cbn. unfold cat, Cat_Kleisli. cbn. *)
-(*         rewrite bind_bind. *)
-(*         apply Proper_bind. *)
-(*         * reflexivity. *)
-(*         * repeat red. destruct a2. *)
-(*           cbn. *)
-(*           rewrite bind_ret_l. reflexivity. *)
-(*   Qed. *)
-
-(*   Lemma internalize_pure_iso {a b c} (f : Kleisli (stateT S m) a (b + c)) : *)
-(*     ((internalize f) >>> pure iso) ⩯ (fun sa => (bind (f (snd sa) (fst sa))) (fun sbc => ret (iso sbc))). *)
-(*   Proof. *)
-(*     reflexivity. *)
-(*   Qed. *)
-
-(*   Lemma eq2_to_eqm : forall a b (f g : Kleisli (stateT S m) a b) (x:a) (s:S), *)
-(*       eq2 f g -> *)
-(*       eqm (f x s) (g x s). *)
-(*   Proof. *)
-(*     intros a b f g x s H. *)
-(*     specialize (H x s). rewrite prod_rel_eq in H. *)
-(*     apply H. *)
-(*   Qed. *)
-
-(*   Lemma iter_dinatural_helper: *)
-(*     forall (a b c : Type) (f : Kleisli (stateT S m) a (b + c)) (g : Kleisli (stateT S m) b (a + c)), *)
-(*       internalize (f >>> case_ g inr_) >>> pure iso ⩯ internalize f >>> pure iso >>> case_ (internalize g >>> pure iso) inr_. *)
-(*   Proof. *)
-(*     destruct Cm. *)
-(*     intros a b c f g. *)
-(*     repeat red. *)
-(*     destruct a0. *)
-(*     unfold cat, Cat_Kleisli, internalize. *)
-(*     cbn. *)
-(*     repeat rewrite bind_bind. *)
-(*     apply Proper_bind. *)
-(*     - reflexivity. *)
-(*     - repeat red. *)
-(*       destruct a1 as [s' [x | y]]. *)
-(*       + unfold pure. *)
-(*         rewrite bind_ret_l. *)
-(*         unfold case_, Case_Kleisli, Function.case_sum. *)
-(*         reflexivity. *)
-(*       + unfold pure. rewrite bind_ret_l. *)
-(*         unfold case_, Case_Kleisli, Function.case_sum. *)
-(*           cbn. *)
-(*           rewrite bind_ret_l. reflexivity. *)
-(*   Qed. *)
-
-
-(*   Global Instance IterDinatural_stateT : IterDinatural (Kleisli (stateT S m)) sum. *)
-(*   Proof. *)
-(*     destruct Cm. *)
-(*     unfold IterDinatural. *)
-(*     repeat red. *)
-(*     intros a b c f g a0 a1. *)
-(*     unfold iter, Iter_stateT. *)
-(*     eapply transitivity. rewrite prod_rel_eq. *)
-(*     eapply iterative_proper_iter. *)
-(*     apply iter_dinatural_helper. *)
-(*     rewrite iterative_dinatural. *)
-(*     cbn. *)
-(*     unfold cat, Cat_Kleisli. *)
-(*     rewrite bind_bind. *)
-(*     unfold internalize. cbn. rewrite prod_rel_eq. *)
-(*     apply Proper_bind. *)
-(*     - reflexivity. *)
-(*     - repeat red. *)
-(*       destruct a2 as [s [x | y]]. *)
-(*       + unfold pure. *)
-(*         rewrite bind_ret_l. *)
-(*         cbn. *)
-(*         eapply iterative_proper_iter. *)
-(*         repeat red. *)
-(*         destruct a2. *)
-(*         cbn. rewrite! bind_bind. *)
-(*         apply Proper_bind. *)
-(*         * reflexivity. *)
-(*         * repeat red. *)
-(*           destruct a2 as [s' [x' | y]]. *)
-(*           ** cbn.  rewrite bind_ret_l. unfold case_, Case_Kleisli, Function.case_sum. *)
-(*              reflexivity. *)
-(*           ** cbn.  rewrite bind_ret_l. unfold case_, Case_Kleisli, Function.case_sum. *)
-(*              rewrite bind_ret_l. reflexivity. *)
-(*       + unfold pure. *)
-(*         rewrite bind_ret_l. *)
-(*         cbn. *)
-(*         reflexivity. *)
-(*     Qed. *)
-
-
-(*   Global Instance IterCodiagonal_stateT : IterCodiagonal (Kleisli (stateT S m)) sum. *)
-(*   Proof. *)
-(*     destruct Cm. *)
-(*     unfold IterCodiagonal. *)
-(*     intros a b f. *)
-(*     unfold iter, Iter_stateT. *)
-(*     repeat red. *)
-(*     intros. *)
-(*     eapply transitivity. rewrite prod_rel_eq. *)
-(*     eapply iterative_proper_iter. *)
-(*     eapply Proper_cat_Kleisli. *)
-
-(*     assert (internalize (fun (x:a) (s:S) => iter (internalize f >>> pure iso) (s, x)) *)
-(*                        ⩯ *)
-(*                        iter (internalize f >>> pure iso)). *)
-(*     { repeat red. *)
-(*       intros a2. *)
-(*       destruct a2. *)
-(*       unfold internalize. *)
-(*       cbn.  reflexivity. *)
-(*     } *)
-(*    apply H. *)
-(*    reflexivity. *)
-(*    eapply transitivity. rewrite prod_rel_eq. *)
-
-(*    eapply iterative_proper_iter. *)
-(*    apply iterative_natural. *)
-(*    rewrite iterative_codiagonal. rewrite prod_rel_eq. *)
-(*    eapply iterative_proper_iter. *)
-(*    rewrite internalize_cat. *)
-(*    (* SAZ This proof can probably use less unfolding *) *)
-(*    repeat red. intros a2. *)
-(*    destruct a2. *)
-(*    unfold cat, Cat_Kleisli. cbn. *)
-(*    repeat rewrite bind_bind. *)
-(*    unfold internalize, pure. *)
-(*    cbn. *)
-(*    apply Proper_bind. *)
-(*     - reflexivity. *)
-(*     - repeat red. *)
-(*       intros a3. *)
-(*       destruct a3 as [s' [x | [y | z]]]. *)
-(*       + rewrite bind_ret_l. *)
-(*         cbn. unfold id_, Id_Kleisli, pure. *)
-(*         rewrite bind_ret_l. *)
-(*         unfold cat, Cat_Kleisli. *)
-(*         rewrite bind_bind. *)
-(*         rewrite bind_ret_l. *)
-(*         cbn.  unfold inl_, Inl_Kleisli, pure. *)
-(*         rewrite bind_ret_l. reflexivity. *)
-(*       + rewrite bind_ret_l. *)
-(*         cbn. *)
-(*         rewrite bind_ret_l. *)
-(*         unfold cat, Cat_Kleisli. *)
-(*         rewrite bind_bind, bind_ret_l. cbn. *)
-(*         unfold inr_, Inr_Kleisli, pure. *)
-(*         rewrite bind_ret_l. reflexivity. *)
-(*       + rewrite bind_ret_l. *)
-(*         cbn. *)
-(*         rewrite bind_ret_l. *)
-(*         unfold cat, Cat_Kleisli. *)
-(*         rewrite bind_bind, bind_ret_l. cbn. *)
-(*         unfold inr_, Inr_Kleisli, pure. *)
-(*         rewrite bind_ret_l. *)
-(*         reflexivity. *)
-(*   Qed. *)
-
-(*   Global Instance Iterative_stateT : Iterative (Kleisli (stateT S m)) sum. *)
-(*   Proof. *)
-(*   constructor; *)
-(*   typeclasses eauto. *)
-(*   Qed. *)
-
-End StateT.
+End State.
