theories/Basics/MonadID.v
@@ -133,6 +133,10 @@ split; intros; unfold ID in *; try tauto.
     apply image_Id in H0. destruct H0 as (HA1 & HA2).
     rewrite HA1. 
     apply H.
+- split. cbn. intros. apply EQ.
+  apply image_Id in H. destruct H.
+  exists ma. intros. apply image_Id in H1.
+  destruct H1. cbn. intros. rewrite H. cbn. apply EQ.
 Qed.
 
 Instance EqmRBindInversion_ID : EqmRBindInversion ID.
